basic so-dec proof and example

src/so.v
@@ -1,11 +1,40 @@
 From mathcomp Require Import all_ssreflect.
 From Paco Require Import paco.
-Require Import ST.src.stream ST.src.st ST.types.local.
+Require Import ST.aux.axioms ST.src.stream ST.src.st ST.types.local.
 Require Import String List.
 Local Open Scope string_scope.
 Import ListNotations.
+Import CoListNotations.
 Require Import Setoid.
 Require Import Morphisms.
+
+CoFixpoint st2soH (t: st): st :=
+match t with
+  | st_send p xs    =>
+    match xs with
+      | cocons (l,s,t') ys => st_send p [|(l,s,st2soH t')|] 
+      | conil              => st_send p conil
+    end
+  | st_receive p xs => 
+      let cofix next xs :=
+      match xs with
+        | cocons (l,s,t') ys => cocons (l,s,st2soH t') (next ys)
+        | conil              => conil
+      end 
+    in st_receive p (next xs) 
+  | _               => st_end
+end.
+
+CoFixpoint st2soF (t: st): coseq st :=
+match t with
+  | st_send p xs => 
+    match xs with
+      | cocons(l,s,t') ys => cocons (st_send p [|(l,s,st2soH t')|]) (st2soF (st_send p ys))
+      | conil             => conil
+    end
+  | _            => [|st2soH t|]
+end.
+
 
 Inductive st2so (R: st -> st -> Prop): st -> st -> Prop :=
   | st2so_end: st2so R st_end st_end
@@ -14,7 +43,7 @@ Inductive st2so (R: st -> st -> Prop): st -> st -> Prop :=
                copathsel l s xs y ->
                st2so R (st_send p (cocons (l,s,x) conil)) (st_send p xs)
   | st2so_rcv: forall p xs ys,
-               Forall2C (fun u v => exists l s t l' s' t', u = (l,s,t) /\ v = (l',s',t') /\ R t t') ys xs ->
+               Forall2Co (fun u v => exists l s t l' s' t', u = (l,s,t) /\ v = (l',s',t') /\ R t t') ys xs ->
                st2so R (st_receive p ys) (st_receive p xs).
 
 Definition st2soC s1 s2 := paco2 (st2so) bot2 s1 s2.
@@ -29,7 +58,114 @@ Proof. unfold monotone2.
          apply LE; easy. easy.
        - specialize (st2so_rcv r'); intro HS.
          apply HS.
-         apply monH2 with (r := r); easy.
+         apply monHo2 with (r := r); easy.
+Qed.
+
+CoFixpoint next (xs: coseq(label*sort*st)) :=
+  match xs with
+    | cocons (l,s,t') ys => cocons (l,s,st2soH t') (next ys)
+    | conil              => conil
+  end.
+
+Lemma next_eq: forall xs, next xs = comap (prod_map (prod_map id id) (st2soH)) xs.
+Proof. intros.
+       apply cext.
+       revert xs.
+       pcofix CIH.
+       intros.
+       pfold.
+       destruct xs.
+       - rewrite(coseq_eq(comap (prod_map (prod_map id id) st2soH) [||])). simpl.
+         rewrite(coseq_eq( (next [||]))). simpl. constructor.
+         rewrite(coseq_eq(next (cocons p xs))).
+         rewrite(coseq_eq(comap (prod_map (prod_map id id) st2soH) (cocons p xs))). simpl.
+         destruct p as ((l1,s1),t1).
+         constructor.
+         right. apply CIH.
+         simpl. easy.
+Qed.
+
+Lemma st2soE: forall T, wfC T -> st2soC (st2soH T) T.
+Proof. pcofix CIH.
+       intros T Hwf.
+       case_eq T; intros.
+       - pfold. rewrite(st_eq (st2soH (end))). simpl. constructor.
+       - rewrite(st_eq( (st2soH (s & c)))). simpl.
+         fold next.
+         rewrite next_eq.
+         rewrite(coseq_eq(comap (prod_map (prod_map id id) st2soH) c)). simpl.
+         destruct c. pfold. constructor. pfold. constructor.
+         destruct p as ((l1,s1),t1). simpl.
+         pfold. constructor. pfold.
+         constructor.
+         exists l1. exists s1. exists (st2soH t1).
+         exists l1. exists s1. exists t1.
+         split. easy. split. easy. right. apply CIH.
+         subst.
+         pinversion Hwf. subst.
+         pinversion H2. subst.
+         pfold. destruct H3 as (l2,(s2,(t2,(Ha,Hb)))).
+         inversion Ha. subst.
+         destruct Hb. pinversion H.
+         apply mon_wfH. easy.
+         apply mon_fHo.
+         apply mon_wfH.
+         left. subst.
+         revert c Hwf.
+         pcofix CIH2. intros.
+         case_eq c; intros.
+         rewrite(coseq_eq (comap (prod_map (prod_map id id) st2soH) [||])). simpl.
+         simpl. pfold. constructor.
+         pfold. 
+         rewrite(coseq_eq(comap (prod_map (prod_map id id) st2soH) (cocons p c0))). simpl.
+         constructor.
+         destruct p as ((l2,s2),t2). simpl.
+         exists l2. exists s2. exists (st2soH t2).
+         exists l2. exists s2. exists t2.
+         split. easy. split. easy. right. apply CIH.
+         subst. pinversion Hwf. subst.
+         pinversion H2. subst.
+         pfold.
+         destruct H3 as (l3,(s3,(t3,(Hc,Hd)))).
+         pinversion H4. subst.
+         destruct H3 as (l4,(s4,(t4,(He,Hf)))).
+         inversion He. subst.
+         destruct Hf. pinversion H.
+         apply mon_wfH. easy.
+         apply mon_fHo. apply mon_fHo.
+         apply mon_wfH.
+         right. apply CIH2.
+         subst.
+         pinversion Hwf. subst.
+         pinversion H2. subst.
+         pfold.
+         constructor. easy. pfold.
+         constructor.
+         destruct H3 as (l2,(s2,(t2,(Ha,Hb)))).
+         inversion Ha. subst.
+         exists l2. exists s2. exists t2.
+         split. easy. easy.
+         pinversion H4.
+         subst.
+         left. easy.
+         apply mon_fHo.
+         apply mon_fHo.
+         apply mon_wfH.
+       - rewrite(st_eq( (st2soH (s ! c)))). simpl.
+         destruct c. pfold.
+         subst. pinversion Hwf. easy.
+         apply mon_wfH.
+         subst. 
+         destruct p. destruct p.
+         pfold. apply st2so_snd with (y := s0). right. apply CIH.
+         pinversion Hwf. subst. pinversion H2. subst.
+         destruct H3 as (l3,(s3,(t3,(Ha,Hb)))).
+         inversion Ha. subst.
+         pfold.
+         destruct Hb. pinversion H. apply mon_wfH. easy.
+         apply mon_fHo.
+         apply mon_wfH.
+         constructor.
 Qed.
 
 (*example so decomposition*)
@@ -39,11 +175,6 @@ CoFixpoint Et2 := st_send "q" (cocons ("l8", sint, Et2) conil).
 CoFixpoint Et1so := st_receive "q" (cocons ("l7", sint, Et1so) conil).
 CoFixpoint Et2so := st_send "q" (cocons ("l8", sint, Et2so) conil).
 
-Check (cocons("l4",sint,st_end) 
-                                                    (cocons ("l5",sint,st_end) 
-                                                    (cocons("l6",sint,st_end) 
-                                                    conil))).
-
 CoFixpoint eT1 := st_receive "p" (cocons ("l1",sint,st_send "p" (cocons("l4",sint,Et1) 
                                                                 (cocons ("l5",sint,Et2) 
                                                                 (cocons("l6",sint,eT1) 
@@ -51,7 +182,7 @@ CoFixpoint eT1 := st_receive "p" (cocons ("l1",sint,st_send "p" (cocons("l4",sin
                                  (cocons ("l2",sint,st_send "q" (cocons ("l9",sint,eT1) conil))
                                  (cocons ("l3",sint,st_receive "q" (cocons ("l10",sint,eT1) conil)) conil))).
 
-CoFixpoint eT2 := st_receive "p" (cocons ("l1",sint,st_send "p" (cocons("l4",sint,Et1so) conil)) 
+CoFixpoint eT2 := st_receive "p" (cocons ("l1",sint,st_send "p" (cocons("l4",sint,Et1so) conil))
                                  (cocons ("l2",sint,st_send "q" (cocons ("l9",sint,eT2) conil))
                                  (cocons ("l3",sint,st_receive "q" (cocons ("l10",sint,eT2) conil)) conil))).
 
@@ -59,7 +190,7 @@ Lemma T1soT2: st2soC eT2 eT1.
 Proof. pcofix CIH.
        rewrite(st_eq eT1); rewrite(st_eq eT2); simpl.
        pfold.
-       apply st2so_rcv.
+       apply st2so_rcv. pfold.
        constructor.
 
        exists "l1". exists (I). exists ("p" ! cocons ("l4", I, Et1so) conil).
@@ -71,43 +202,35 @@ Proof. pcofix CIH.
        left.
        pcofix CIH2.
        rewrite(st_eq Et1). simpl. rewrite(st_eq Et1so). simpl.
-       pfold. apply st2so_rcv.
+       pfold. apply st2so_rcv. pfold.
        constructor.
-
        exists "l7". exists (I). exists (Et1so).
        exists "l7". exists (I). exists (Et1).
        split. easy. split. easy. right. easy.
-       constructor.
-       constructor.
+       constructor. pfold.
+       constructor. 
 
-       constructor.
+       constructor. left. pfold. constructor.
        exists "l2". exists (I). exists ("q" ! cocons ("l9", I, eT2) conil).
        exists "l2". exists (I). exists ("q" ! cocons ("l9", I, eT1) conil).
        split. easy. split. easy.
        left. pfold. apply st2so_snd with (y := eT1).
        right. easy.
        constructor.
-       
 
-       constructor.
+       constructor. pfold. constructor.
        exists "l3". exists (I). exists ("q" & cocons ("l10", I, eT2) conil).
        exists "l3". exists (I). exists ("q" & cocons ("l10", I, eT1) conil).
        split. easy. split. easy.
-       left. pfold. apply st2so_rcv.
-       constructor.
+       left. pfold. apply st2so_rcv. pfold.
+       constructor. 
 
        exists "l10". exists (I). exists (eT2).
        exists "l10". exists (I). exists (eT1).
        split. easy. split. easy. right. easy.
-       
+
+       constructor. pfold.
        constructor.
-       constructor.
+       left. pfold. constructor.
 Qed.
-
-
-
-
-
-
-
 
